mechanization/theories/Core/Completeness/LogicalRelation/Definitions.v
@@ -27,6 +27,22 @@ Hint Transparent valid_exp_under_ctx : mcpts.
 #[export]
 Hint Unfold valid_exp_under_ctx : mcpts.
 
+Definition rel_typ_under_ctx {P} (pred_P : PredicativeSig P) (Γ : ctx P) A A' :=
+  exists env_rel,
+    {{ EF Γ ≈ Γ ∈ per_ctx_env pred_P ↘ env_rel }} /\
+      forall ρ ρ' (equiv_ρ_ρ' : {{ Dom ρ ≈ ρ' ∈ env_rel }}),
+      exists (elem_rel : relation (domain P)),
+        rel_typ_unsorted pred_P A ρ A' ρ' elem_rel.
+
+Definition valid_typ_under_ctx {P} {pred_P : PredicativeSig P} Γ A := rel_typ_under_ctx pred_P Γ A A.
+#[global]
+Arguments valid_typ_under_ctx {_} _ _ _ /.
+#[export]
+Hint Transparent valid_typ_under_ctx : mcpts.
+#[export]
+Hint Unfold valid_typ_under_ctx : mcpts.
+              
+
 Inductive rel_sub {P : PtsSig} σ ρ σ' ρ' (R : relation (env P)) : Prop :=
 | mk_rel_sub : forall ρσ ρ'σ', {{ ⟦ σ ⟧s ρ ↘ ρσ }} -> {{ ⟦ σ' ⟧s ρ' ↘ ρ'σ' }} -> {{ Dom ρσ ≈ ρ'σ' ∈ R }} -> rel_sub σ ρ σ' ρ' R.
 #[global]
@@ -54,5 +70,7 @@ Notation "⟪ pred_P ⟫ ⊨ Γ ≈ Γ'" := (per_ctx pred_P Γ Γ')  (in custom 
 Notation "⟪ pred_P ⟫ ⊨ Γ" := (valid_ctx pred_P Γ) (in custom judg at level 80, pred_P constr at level 0, Γ custom exp).
 Notation "⟪ pred_P ⟫ Γ ⊨ M ≈ M' : A" := (rel_exp_under_ctx pred_P Γ A M M') (in custom judg at level 80, pred_P constr at level 0, Γ custom exp, M custom exp, M' custom exp, A custom exp).
 Notation "⟪ pred_P ⟫ Γ ⊨ M : A" := (valid_exp_under_ctx pred_P Γ A M) (in custom judg at level 80, pred_P constr at level 0, Γ custom exp, M custom exp, A custom exp).
+Notation "⟪ pred_P ⟫ Γ ⊨ A ≈ A'" := (rel_typ_under_ctx pred_P Γ A A') (in custom judg at level 80, pred_P constr at level 0, Γ custom exp, A custom exp, A' custom exp).
+Notation "⟪ pred_P ⟫ Γ ⊨ A" := (valid_typ_under_ctx pred_P Γ A) (in custom judg at level 80, pred_P constr at level 0, Γ custom exp, A custom exp).
 Notation "⟪ pred_P ⟫ Γ ⊨s σ ≈ σ' : Δ" := (rel_sub_under_ctx pred_P Γ Δ σ σ') (in custom judg at level 80, pred_P constr at level 0, Γ custom exp, σ custom exp, σ' custom exp, Δ custom exp).
 Notation "⟪ pred_P ⟫ Γ ⊨s σ : Δ" := (valid_sub_under_ctx pred_P Γ Δ σ) (in custom judg at level 80, pred_P constr at level 0, Γ custom exp, σ custom exp, Δ custom exp).
